LivenessAnalysisCorrect.v
@@ -128,3 +128,32 @@ Proof.
       rewrite <- H17.
       rewrite <- H13. reflexivity.
 Qed.
+
+Definition livenessAnalysis s :=
+  let a := Analysis.safeFixpoint (LivenessAnalysis.liveness_analysis s) in
+  mapAnn (@proj1_sig _ _) (proj1_sig (proj1_sig a)).
+
+
+
+Ltac destr_sig H :=
+  match type of H with
+  | context [proj1_sig ?x] => destruct x; simpl in H
+  end.
+
+Tactic Notation "destr_sig" :=
+  match goal with
+  | [ |- context [proj1_sig (proj1_sig ?x)] ] => destruct x; simpl
+  | [ |- context [proj1_sig ?x] ] => destruct x; simpl
+  end.
+
+Definition correct s
+  : labelsDefined s 0
+    -> paramsMatch s nil
+    -> true_live_sound Imperative nil nil s (livenessAnalysis s).
+Proof.
+  intros.
+  unfold livenessAnalysis.
+  destr_sig. destr_sig. dcr.
+  eapply (@liveness_analysis_correct s nil nil s); eauto.
+  eapply H3.
+Qed.
