Equiv/BisimSim.v
@@ -30,3 +30,29 @@ Proof.
     + intros. edestruct H7; eauto; dcr. eexists; eauto.
   - econstructor 3; eauto.
 Qed.
+
+Lemma bisim_sim' {S1} `{StateType S1}
+      (σ1:S1) {S2} `{StateType S2} (σ2:S2)
+  : Sim.sim Bisim σ1 σ2 -> Sim.sim Sim σ1 σ2.
+Proof.
+  revert σ1 σ2. cofix; intros.
+  inv H1.
+  - econstructor; eauto.
+  - econstructor 2; eauto.
+    + intros. edestruct H6; eauto; dcr. eexists; eauto.
+    + intros. edestruct H7; eauto; dcr. eexists; eauto.
+  - econstructor 4; eauto.
+Qed.
+
+Lemma sim_sym {S1} `{StateType S1}
+      (σ1:S1) {S2} `{StateType S2} (σ2:S2)
+  : Sim.sim Bisim σ1 σ2 -> Sim.sim Bisim σ2 σ1.
+Proof.
+  revert σ1 σ2. cofix; intros.
+  inv H1.
+  - econstructor; eauto.
+  - econstructor 2; eauto.
+    + intros. edestruct H7; eauto; dcr. eexists; eauto.
+    + intros. edestruct H6; eauto; dcr. eexists; eauto.
+  - econstructor 4; eauto.
+Qed.
